utilities.v
@@ -215,6 +215,7 @@ Proof. by rewrite seq_inE mem_pmap_sub. Qed.
 
 End SeqIn.
 
+
 (* ************************************************************************** *)
 (*     Missing definitions, notations and lemmas for Relation Algebra          *)
 (* ************************************************************************** *)
@@ -410,3 +411,14 @@ Qed.
 End RelationOnSeq.
 
 
+Section OptionUtils. 
+
+Context {T rT : Type}.
+
+Definition opreim (f : T -> option rT) (p : pred rT) : simpl_pred T := 
+  [pred x | match f x with Some x => p x | _ => false end]. 
+
+Definition orelpre (f : T -> option rT) (r : rel rT) : simpl_rel T := 
+  [rel x y | match f x, f y with Some x, Some y => r x y | _, _ => false end].
+
+End OptionUtils.
